major updates to extension_proof.v to support effect-based formulation of rely-guarantee conditions.  the proof now builds but with a bunch of (hopefully minor) holes (which i'll attempt to fill over the next few days).
one hole, related to pointers received from the environment, may require
an additional condition in the after-external case of the simulation 
diagram.  

the proof has also been updated to eliminate the need for 'stable' 
rely-guarantee simulations, by ensuring that cores that are not 
'focused' -- i.e., actively running in the context of a given extension -- 
are blocked at-external.  this will be true both of the linking semantics
and of our nonpreemptive concurrency semantics.

also: add a coinductive formulation of "compile_safe"

other updates include: 
-removing 'Load loadpath' commands in various places
-probably some other minor stuff...

sepcomp-reserved/compile_safe.v
@@ -14,7 +14,7 @@ Definition is_ptr (v: val) := exists b ofs, v = Vptr b ofs.
 (* can't define as a fixpoint because there may be cycles *)
 
 Inductive ptr_closure (b: block) (ofs: Z) (m: mem): block -> Z -> Prop :=
-| ptr_closure_base: ptr_closure b ofs m b ofs
+| ptr_closure_base: forall ofs', ptr_closure b ofs m b ofs'
 | ptr_closure_trans: forall b'' ofs'' b' ofs',
   Mem.load Mint32 m b ofs = Some (Vptr b'' ofs'') -> 
   ptr_closure b'' (Int.intval ofs'') m b' ofs' -> 
@@ -27,7 +27,7 @@ Definition closure (v: val) (m: mem): val -> Prop :=
                    | _, _ => False
                  end.
 
-Definition val_not_reserved (v: option val) (m: mem) (r: reserve_map) :=
+Definition val_not_reserved (v: option val) (m: mem) (r: reserve) :=
   match v with Some v' => 
     forall b ofs, closure v' m (Vptr b ofs) -> ~r b (Int.intval ofs)
   | None => True
@@ -47,17 +47,42 @@ solve[econstructor].
 solve[auto].
 Qed.
 
-Definition reserve_separated1 (r r': reserve_map) m := 
+(*TODO: move elsewhere*)
+Definition reserve_separated1 (r r': reserve) m := 
   forall b ofs, ~r b ofs -> r' b ofs -> ~Mem.valid_block m b.
 
 Section compile_safety.
   Context {G C D Z:Type}.
-  Context (Hcore:RelyGuaranteeSemantics G C D).
-  Variable (Hspec:external_specification mem external_function Z).
+  Context (Hcore:EffectfulSemantics G C D).
 
   Variable ge : G.
 
-  Fixpoint compile_safeN (n:nat) (z:Z) (r:reserve_map) (c:C) (m:mem) : Prop :=
+  CoInductive compile_safe: Z -> reserve -> C -> mem -> Prop :=
+  | compile_safe_halt: 
+    forall z r c m ret, 
+    safely_halted Hcore c = Some ret -> 
+    val_not_reserved (Some ret) m r -> 
+    compile_safe z r c m
+  | compile_safe_step:
+    forall z (r: reserve) c m (r': reserve) c' m',
+    reserve_incr r r' -> 
+    reserve_separated1 r r' m -> 
+    guarantee Hcore r' c' m' -> 
+    corestep Hcore ge c m c' m' -> 
+    compile_safe z r' c' m' -> 
+    compile_safe z r c m
+  | compile_safe_external: 
+    forall z (r: reserve) c m e sig args, 
+     at_external Hcore c = Some (e, sig, args) -> 
+    (forall z' (r': reserve) c' m' ret,
+     reserve_incr r r' -> 
+     reserve_separated1 r r' m -> 
+     val_not_reserved ret m' r' -> 
+     after_external Hcore ret c = Some c' -> 
+     compile_safe z' r' c' m') ->  
+    compile_safe z r c m.
+
+  Fixpoint compile_safeN (n:nat) (z:Z) (r:reserve) (c:C) (m:mem) : Prop :=
     match n with
     | O => True
     | S n' => 
@@ -65,11 +90,14 @@ Section compile_safety.
        | None, None =>
            forall c' m', 
              corestep Hcore ge c m c' m' -> 
-             mem_unchanged_on (guarantee_left Hcore r c) m m' /\ 
-             compile_safeN n' z r c' m'
+             exists r': reserve, 
+               reserve_incr r r' /\
+               reserve_separated1 r r' m /\
+               guarantee Hcore r' c' m' /\ 
+               compile_safeN n' z r' c' m'
        | Some (e,sig,args), None =>
-           forall ret m' z' r' c',
-             reserve_map_incr r r' -> 
+           forall ret m' z' (r': reserve) c',
+             reserve_incr r r' -> 
              reserve_separated1 r r' m -> 
              val_not_reserved ret m' r' -> 
              after_external Hcore ret c = Some c' -> 
@@ -79,23 +107,66 @@ Section compile_safety.
        end
     end.
 
+  Definition compile_safe' z r c m := forall n, compile_safeN n z r c m.
+
   Definition corestep_fun  :=
        forall ge m q m1 q1 m2 q2 ,
        corestep Hcore ge q m q1 m1 -> 
        corestep Hcore ge q m q2 m2 -> 
        (q1, m1) = (q2, m2).
 
+  Lemma compile_safe_safe': 
+    forall z r c m,
+    corestep_fun -> 
+    compile_safe z r c m -> compile_safe' z r c m.
+  Proof.
+  intros until m; intros FUN H1 n.
+  revert z r c m H1.
+  induction n; intros; hnf; auto.
+  case_eq (at_external Hcore c).
+  intros [[ef sig] args] H2.
+  case_eq (safely_halted Hcore c).
+  intros v H3.
+  exploit @at_external_halted_excl.
+  instantiate (1 := c).
+  instantiate (1 := Hcore).
+  rewrite H2, H3.
+  intros [?|?]; congruence.
+  intros NONE.
+  intros.
+  apply IHn.
+  inv H1; try solve[congruence].
+  apply corestep_not_at_external in H8.
+  congruence.
+  solve[eapply H6; eauto].
+  intros NONE.
+  case_eq (safely_halted Hcore c).
+  intros v HALT.
+  inv H1; try solve[congruence].
+  solve[rewrite H in HALT; inv HALT; auto].
+  exploit @corestep_not_halted; eauto; intros.
+  congruence.
+  intros NONE'.
+  intros until m'; intros H2.
+  inv H1; try solve[congruence].
+  generalize (FUN _ _ _ _ _ _ _ H2 H4); intros X.
+  inv X; exists r'; split; auto.
+  Qed.
+
   Lemma compile_safe_corestep_forward:
     corestep_fun -> 
     forall c m c' m' n z r,
     corestep Hcore ge c m c' m' -> 
     compile_safeN (S n) z r c m -> 
-    compile_safeN n z r c' m'.
+    exists r': reserve, 
+      reserve_incr r r' /\
+      reserve_separated1 r r' m /\
+      guarantee Hcore r' c' m' /\ 
+      compile_safeN n z r' c' m'.
   Proof.
-    simpl; intros.
-    erewrite corestep_not_at_external in H1; eauto.
-    erewrite corestep_not_halted in H1; eauto.
-    solve[destruct (H1 c' m') as [H2 H3]; auto].
+  simpl; intros.
+  erewrite corestep_not_at_external in H1; eauto.
+  erewrite corestep_not_halted in H1; eauto.
   Qed.
 
   Lemma compile_safe_downward1 :
@@ -112,7 +183,8 @@ Section compile_safety.
     auto.
     intros.
     exploit H; eauto.
-    solve[intros [? ?]; auto].
+    intros [r' [? [? [? ?]]]].
+    solve[exists r'; split; auto].
   Qed.
 
   Lemma compile_safe_downward: 
@@ -125,3 +197,5 @@ Section compile_safety.
   Qed.
     
 End compile_safety.
+
+
