sepcomp-reserved/extension_proof.v
@@ -2,6 +2,7 @@ Require Import sepcomp.mem_lemmas.
 Require Import sepcomp.core_semantics.
 Require Import sepcomp.forward_simulations. 
 Require Import sepcomp.rg_forward_simulations. 
+Require Import sepcomp.compile_safe.
 Require Import sepcomp.step_lemmas. 
 Require Import sepcomp.extspec. 
 Require Import sepcomp.extension.
@@ -25,7 +26,8 @@ Tactic Notation "remember" constr(a) "as" ident(x) :=
   let H := fresh "Heq" x in
   (set (x:=a) in *; assert (H: x=a) by reflexivity; clearbody x).
 
-(*TODO: move this lemma somewhere above extension_proof.v and extension_proof_safety.v*)
+(*TODO: move this lemma somewhere above extension_proof.v and 
+   extension_proof_safety.v*)
 Lemma runnable_false (G C M D: Type) (csem: CoreSemantics G C M D): 
  forall c, runnable csem c=false -> 
  (exists rv, safely_halted csem c = Some rv) \/
@@ -51,12 +53,13 @@ Section CoreCompatibleLemmas. Variables
  (G: Type) (** global environments of extended semantics *)
  (D: Type) (** extension initialization data *)
  (xT: Type) (** corestates of extended semantics *)
- (esem: RelyGuaranteeSemantics G xT D) (** extended semantics *)
+ (esem: EffectfulSemantics G xT D) (** extended semantics *)
  (esig: ef_ext_spec mem Zext) (** extension signature *)
  (gT: nat -> Type) (** global environments of core semantics *)
  (dT: nat -> Type) (** initialization data *)
  (cT: nat -> Type) (** corestates of core semantics *)
- (csem: forall i:nat, RelyGuaranteeSemantics (gT i) (cT i) (dT i)) (** a set of core semantics *)
+(** a set of core semantics *)
+ (csem: forall i:nat, EffectfulSemantics (gT i) (cT i) (dT i)) 
  (csig: ef_ext_spec mem Z). (** client signature *)
 
  Variables (ge: G) (genv_map : forall i:nat, gT i).
@@ -163,13 +166,13 @@ assert (H6: Mem.nextblock m <= Mem.nextblock m').
  solve[apply forward_nextblock in H3; auto].
 destruct (eq_nat_dec i (active E s)). subst.
 rewrite PROJ in H5; inv H5.
-assert (H5: {owned (csem (active E s)) x b ofs}+
-            {~owned (csem (active E s)) x b ofs}) 
- by apply owned_dec.
+assert (H5: {effects (csem (active E s)) x AllocEffect b ofs}+
+            {~effects (csem (active E s)) x AllocEffect b ofs}) 
+ by apply effects_dec.
 destruct H5 as [H5|H5].
 specialize (H2 (active E s) x H1 b ofs H5).
 omega.
-eapply owned_newN in PRIV; eauto.
+eapply effects_newN in PRIV; eauto.
 solve[destruct PRIV; auto].
 
 cut (proj_core E i s = Some x''). intro H7.
@@ -184,10 +187,11 @@ solve[erewrite corestep_others_backward; eauto].
 Qed.
 
 Lemma owned_dec: forall i x b ofs,
-  {owned (csem i) x b ofs}+{~owned (csem i) x b ofs}.
+  {effects (csem i) x AllocEffect b ofs}+
+  {~effects (csem i) x AllocEffect b ofs}.
 Proof.
 intros.
-apply owned_dec; auto.
+apply effects_dec; auto.
 Qed.
 
 Lemma owned_valid_after_ext: 
@@ -213,7 +217,8 @@ omega.
 solve[apply forward_nextblock in FWD; auto].
 eapply PRIV; eauto.
 rewrite PROJC in PROJ'; inv PROJ'.
-eapply owned_external in AFTER; eauto.
+eapply effects_external in AFTER; eauto.
+destruct AFTER.
 solve[elimtype False; eauto].
 assert (proj_core E i s = Some c).
  inv Hcore_compatible.
@@ -243,7 +248,7 @@ destruct (eq_nat_dec i (active E s)).
 subst.
 rewrite PROJ' in PROJC.
 inv PROJC.
-eapply owned_external in PRIVATE; eauto.
+eapply effects_external in PRIVATE; eauto.
 inv Hcore_compatible.
 eapply after_ext_others in AFTER'; eauto.
 rewrite <-AFTER' in *; clear AFTER'.
@@ -252,7 +257,7 @@ destruct (eq_nat_dec j (active E s)).
 subst.
 rewrite PROJ' in PROJD.
 inv PROJD.
-eapply owned_external in CONTRA; eauto.
+eapply effects_external in CONTRA; eauto.
 inv Hcore_compatible.
 apply after_ext_others with (j := i) in AFTER'; eauto.
 rewrite <-AFTER' in *; clear AFTER'.
@@ -283,11 +288,11 @@ destruct (eq_nat_dec i (active E s)). subst.
 cut (proj_core E j s = Some d). intro H9.
 rewrite H5 in H7; inv H7.
 intros b ofs H7 CONTRA.
-assert (H10: ~owned (csem (active E s)) x b ofs).
+assert (H10: ~effects (csem (active E s)) x AllocEffect b ofs).
 assert (Hneq: j<>active E s) by auto.
  solve[apply (H2 j (active E s) d x Hneq H9 H1); auto].
 generalize H3 as H3'; intro.
-eapply owned_newN in H3; eauto.
+eapply effects_newN in H3; eauto.
 specialize (VAL j d H9 b ofs CONTRA).
 omega.
 inv Hcore_compatible.
@@ -296,11 +301,11 @@ destruct (eq_nat_dec j (active E s)). subst.
 cut (proj_core E i s = Some c). intro H9.
 rewrite H5 in H8; inv H8.
 intros b ofs H8 CONTRA.
-assert (H10: ~owned (csem (active E s)) x b ofs).
+assert (H10: ~effects (csem (active E s)) x AllocEffect b ofs).
 assert (Hneq: i<>active E s) by auto.
  solve[apply (H2 i (active E s) c x Hneq H9 H1); auto].
 generalize H3 as H3'; intro.
-eapply owned_newN in H3; eauto.
+eapply effects_newN in H3; eauto.
 specialize (VAL i c H9 b ofs H8).
 omega.
 inv Hcore_compatible.
@@ -412,6 +417,8 @@ exists Tfloat; simpl; auto.
 exists Tint; simpl; auto.
 Qed.
 
+Notation allocs_shrink := CompilabilityInvariant.allocs_shrink.
+
 Module ExtendedSimulations. Section ExtendedSimulations.
  Variables
   (F_S V_S F_T V_T: Type) (** source and target extension global environments *)
@@ -423,14 +430,14 @@ Module ExtendedSimulations. Section ExtendedSimulations.
   (Z: Type) (** external states *)
   (Zint: Type) (** portion of Z implemented by extension *)
   (Zext: Type) (** portion of Z external to extension *)
-  (esemS: RelyGuaranteeSemantics (Genv.t F_S V_S) xS D_S) (** extended source semantics *)
-  (esemT: RelyGuaranteeSemantics (Genv.t F_T V_T) xT D_T) (** extended target semantics *)
+  (esemS: EffectfulSemantics (Genv.t F_S V_S) xS D_S) (** extended source semantics *)
+  (esemT: EffectfulSemantics (Genv.t F_T V_T) xT D_T) (** extended target semantics *)
  (** a set of core semantics *)
   (csemS: forall i:nat, 
-    RelyGuaranteeSemantics (Genv.t (fS i) (vS i)) (cS i) (dS i)) 
+    EffectfulSemantics (Genv.t (fS i) (vS i)) (cS i) (dS i)) 
  (** a set of core semantics *)
   (csemT: forall i:nat, 
-    RelyGuaranteeSemantics (Genv.t (fT i) (vT i)) (cT i) (dT i)) 
+    EffectfulSemantics (Genv.t (fT i) (vT i)) (cT i) (dT i)) 
   (csig: ef_ext_spec mem Z) (** client signature *)
   (esig: ef_ext_spec mem Zext) (** extension signature *)
   (threads_max: nat).
@@ -456,7 +463,7 @@ Module ExtendedSimulations. Section ExtendedSimulations.
 
  Variable core_data: forall i: nat, Type.
  Variable match_state: forall i: nat, 
-   core_data i -> reserve_map -> meminj -> cS i -> mem -> cT i -> mem -> Prop.
+   core_data i -> reserve -> meminj -> cS i -> mem -> cT i -> mem -> Prop.
  Variable core_ord: forall i: nat, core_data i -> core_data i -> Prop.
  Implicit Arguments match_state [].
  Implicit Arguments core_ord [].
@@ -469,7 +476,14 @@ Module ExtendedSimulations. Section ExtendedSimulations.
 
  Definition core_datas := forall i:nat, core_data i.
 
- Variable R: reserve_map -> meminj -> xS -> mem -> xT -> mem -> Prop.
+ Variable R: reserve -> meminj -> xS -> mem -> xT -> mem -> Prop.
+
+ (*User proof obligation*)
+ Variable R_antimonotone: 
+   forall (r0 r: reserve) j s1 m1 s2 m2,
+   reserve_incr r0 r -> 
+   R r j s1 m1 s2 m2 -> 
+   R r0 j s1 m1 s2 m2.
 
  Definition core_ords (max_cores: nat) cd1 cd2 := 
 (*exists i, (i < max_cores)%nat /\
@@ -501,51 +515,53 @@ Module ExtendedSimulations. Section ExtendedSimulations.
  solve[intros i; destruct (core_simulations i); auto].
  Qed.
 
- Definition match_states (cd: core_datas) (r: reserve_map) (j: meminj) (s1: xS) m1 (s2: xT) m2 :=
+ Definition match_states (cd: core_datas) (r: reserve) (j: meminj) 
+                         (s1: xS) m1 (s2: xT) m2 :=
    owned_valid esemS csemS E_S s1 m1 /\ owned_disjoint esemS csemS E_S s1 /\ 
    owned_valid esemT csemT E_T s2 m2 /\ owned_disjoint esemT csemT E_T s2 /\
-   reserve_map_valid r m1 /\ reserve_map_valid_right r j m2 /\
+   reserve_valid r m1 /\ reserve_valid' r j m2 /\
+   core_semantics.effects_valid esemS s1 m1 /\ 
+   core_semantics.effects_valid esemT s2 m2 /\
+   mem_wd m1 /\ mem_wd m2 /\
+   guarantee esemS r s1 m1 /\ guarantee' esemT j r s2 m2 /\
+   allocs_shrink esemS esemT j s1 s2 /\
    R r j s1 m1 s2 m2 /\ 
    ACTIVE E_S s1=ACTIVE E_T s2 /\
-   forall i c1, PROJ_CORE E_S i s1 = Some c1 -> 
+   (*invariant on active cores*)
+   (forall c1, 
+     PROJ_CORE E_S (ACTIVE E_S s1) s1 = Some c1 -> 
+     guarantee (csemS (ACTIVE E_S s1)) r c1 m1 /\
+     (exists z: Z, 
+       compile_safe (csemS (ACTIVE E_S s1)) (genv_mapS (ACTIVE E_S s1)) z r c1 m1) /\
+     exists c2, PROJ_CORE E_T (ACTIVE E_S s1) s2 = Some c2 /\ 
+       guarantee' (csemT (ACTIVE E_S s1)) j r c2 m2 /\
+       match_state (ACTIVE E_S s1) (cd (ACTIVE E_S s1)) r j c1 m1 c2 m2) /\
+   (*invariant on inactive cores*)
+   (forall i c1, 
+     i <> ACTIVE E_S s1 -> 
+     PROJ_CORE E_S i s1 = Some c1 -> 
      exists c2, PROJ_CORE E_T i s2 = Some c2 /\ 
-       match_state i (cd i) r j c1 m1 c2 m2.
+     exists cd0 (r0: reserve) j0 m10 m20,
+       guarantee (csemS i) r0 c1 m10 /\
+       (exists z: Z, compile_safe (csemS i) (genv_mapS i) z r0 c1 m10) /\
+       guarantee' (csemT i) j0 r0 c2 m20 /\
+       match_state i cd0 r0 j0 c1 m10 c2 m20).
 
  Variable max_cores: nat. (*TODO: fixme*)
 
  Inductive internal_compilability_invariant: Type := 
-   InternalCompilabilityInvariant: forall 
-  (match_others: forall i cd r r' j j' s1 cd' c1 m1 c1' m1' s2 c2 m2 c2' m2' d1 d2 n, 
-    PROJ_CORE E_S (ACTIVE E_S s1) s1 = Some c1 -> 
-    PROJ_CORE E_T (ACTIVE E_S s1) s2 = Some c2 -> 
-    PROJ_CORE E_S i s1 = Some d1 -> 
-    PROJ_CORE E_T i s2 = Some d2 -> 
-    ACTIVE E_S s1 <> i -> 
-    match_states cd r j s1 m1 s2 m2 -> 
-    Mem.inject j m1 m2 -> 
-    meminj_preserves_globals_ind (genv2blocks ge_S) j -> 
-    inject_incr j j' -> 
-    Events.inject_separated j j' m1 m2 -> 
-    reserve_map_incr r r' -> 
-    reserve_map_separated r r' j' m1 m2 -> 
-    corestep (csemS (ACTIVE E_S s1)) (genv_mapS (ACTIVE E_S s1)) c1 m1 c1' m1' -> 
-    corestepN (csemT (ACTIVE E_S s1)) (genv_mapT (ACTIVE E_S s1)) n c2 m2 c2' m2' -> 
-    match_state (ACTIVE E_S s1) cd' r' j' c1' m1' c2' m2' -> 
-    Events.mem_unchanged_on (guarantee_left (csemS (ACTIVE E_S s1)) r c1) m1 m1' -> 
-    Events.mem_unchanged_on (guarantee_right (csemS (ACTIVE E_S s1)) j r c1) m2 m2' -> 
-    match_state i (cd i) r' j' d1 m1' d2 m2')
+ InternalCompilabilityInvariant: forall 
+ (match_state_runnable: forall i cd r j c1 m1 c2 m2,
+   match_state i cd r j c1 m1 c2 m2 -> runnable (csemS i) c1=runnable (csemT i) c2)
 
-  (match_state_runnable: forall i cd r j c1 m1 c2 m2,
-    match_state i cd r j c1 m1 c2 m2 -> runnable (csemS i) c1=runnable (csemT i) c2)
+ (match_state_inj: forall i cd r j c1 m1 c2 m2,
+   match_state i cd r j c1 m1 c2 m2 -> Mem.inject j m1 m2)
 
-  (match_state_inj: forall i cd r j c1 m1 c2 m2,
-    match_state i cd r j c1 m1 c2 m2 -> Mem.inject j m1 m2)
+ (match_state_preserves_globals: forall i cd r j c1 m1 c2 m2,
+   match_state i cd r j c1 m1 c2 m2 -> 
+   Events.meminj_preserves_globals (genv_mapS i) j)
 
-  (match_state_preserves_globals: forall i cd r j c1 m1 c2 m2,
-    match_state i cd r j c1 m1 c2 m2 -> 
-    Events.meminj_preserves_globals (genv_mapS i) j)
-
- (corestep_rel: forall cd r r' j j' s1 c1 m1 c1' m1' s2 c2 m2 c2' m2' s1' s2' n cd', 
+ (corestep_rel: forall cd (r r': reserve) j j' s1 c1 m1 c1' m1' s2 c2 m2 c2' m2' s1' s2' n cd', 
    PROJ_CORE E_S (ACTIVE E_S s1) s1 = Some c1 -> 
    PROJ_CORE E_T (ACTIVE E_S s1) s2 = Some c2 -> 
    match_states cd r j s1 m1 s2 m2 -> 
@@ -553,28 +569,29 @@ Module ExtendedSimulations. Section ExtendedSimulations.
    meminj_preserves_globals_ind (genv2blocks ge_S) j -> 
    inject_incr j j' -> 
    Events.inject_separated j j' m1 m2 -> 
-   reserve_map_incr r r' -> 
-   reserve_map_separated r r' j' m1 m2 -> 
+   reserve_incr r r' -> 
+   reserve_separated r r' j' m1 m2 -> 
    corestep (csemS (ACTIVE E_S s1)) (genv_mapS (ACTIVE E_S s1)) c1 m1 c1' m1' -> 
    corestepN (csemT (ACTIVE E_S s1)) (genv_mapT (ACTIVE E_S s1)) n c2 m2 c2' m2' ->
    corestep esemS ge_S s1 m1 s1' m1' -> 
    corestepN esemT ge_T n s2 m2 s2' m2' -> 
    match_state (ACTIVE E_S s1) cd' r' j' c1' m1' c2' m2' -> 
-   Events.mem_unchanged_on (guarantee_left (csemS (ACTIVE E_S s1)) r c1) m1 m1' -> 
-   Events.mem_unchanged_on (guarantee_right (csemS (ACTIVE E_S s1)) j r c1) m2 m2' -> 
+   guarantee (csemS (ACTIVE E_S s1)) r c1' m1' -> 
+   guarantee' (csemT (ACTIVE E_S s1)) j r c2' m2' -> 
    R r' j' s1' m1' s2' m2')
 
- (after_external_rel: forall cd r r' j j' s1 m1 s2 m2 s1' m1' s2' m2' ret1 ret2 ef sig args1,
+ (after_external_rel: 
+   forall cd (r r': reserve) j j' s1 m1 s2 m2 s1' m1' s2' m2' ret1 ret2 ef sig args1,
    match_states cd r j s1 m1 s2 m2 -> 
    inject_incr j j' -> 
    Events.inject_separated j j' m1 m2 -> 
-   reserve_map_incr r r' -> 
-   reserve_map_separated r r' j' m1 m2 -> 
+   reserve_incr r r' -> 
+   reserve_separated r r' j' m1 m2 -> 
    Mem.inject j' m1' m2' -> 
    mem_forward m1 m1'-> 
    mem_forward m2 m2' -> 
-   Events.mem_unchanged_on (rely_left esemS r s1) m1 m1' -> 
-   Events.mem_unchanged_on (rely_right esemS j r s1) m2 m2' -> 
+   rely esemS r s1' m1 m1' -> 
+   rely' esemT j r s2' m2 m2' -> 
    at_external esemS s1 = Some (ef, sig, args1) -> 
    after_external esemS ret1 s1 = Some s1' -> 
    after_external esemT ret2 s2 = Some s2' -> 
@@ -582,7 +599,7 @@ Module ExtendedSimulations. Section ExtendedSimulations.
    val_has_type_opt ret2 (ef_sig ef) -> 
    val_inject_opt j' ret1 ret2 -> 
    R r' j' s1' m1' s2' m2')   
- 
+
  (extension_diagram: forall s1 m1 s1' m1' s2 c1 c2 m2 ef sig args1 args2 cd r j,
    PROJ_CORE E_S (ACTIVE E_S s1) s1 = Some c1 -> 
    PROJ_CORE E_T (ACTIVE E_S s1) s2 = Some c2 -> 
@@ -596,14 +613,14 @@ Module ExtendedSimulations. Section ExtendedSimulations.
    Forall2 (val_inject j) args1 args2 -> 
    Forall2 Val.has_type args2 (sig_args (ef_sig ef)) -> 
    corestep esemS ge_S s1 m1 s1' m1' -> 
-   exists s2', exists m2', exists cd', exists r', exists j',
+   guarantee esemS r s1' m1' -> 
+   exists s2', exists m2', exists cd', exists r': reserve, exists j',
      inject_incr j j' /\
      Events.inject_separated j j' m1 m2 /\
-     reserve_map_incr r r' /\
-     reserve_map_separated r r' j' m1 m2 /\
+     reserve_incr r r' /\
+     reserve_separated r r' j' m1 m2 /\
+     guarantee' esemT j' r' s2' m2' /\
      match_states cd' r' j' s1' m1' s2' m2' /\
-     Events.mem_unchanged_on (guarantee_left esemS r s1) m1 m1' /\
-     Events.mem_unchanged_on (guarantee_right esemS j r s1) m2 m2' /\
      ((corestep_plus esemT ge_T s2 m2 s2' m2') \/
       corestep_star esemT ge_T s2 m2 s2' m2' /\ core_ords max_cores cd' cd))
 
@@ -623,20 +640,20 @@ Module ExtendedSimulations. Section ExtendedSimulations.
    at_external esemT s2 = Some (ef, sig, args2))
 
  (after_external_diagram: 
-   forall i d1 s1 m1 d2 s2 m2 s1' m1' s2' m2' ef sig args1 retv1 retv2 cd r r' j j',
+   forall i d1 s1 m1 d2 s2 m2 s1' m1' s2' m2' ef sig args1 retv1 retv2 cd (r r': reserve) j j',
    match_state i cd r j d1 m1 d2 m2 -> 
    at_external esemS s1 = Some (ef, sig, args1) -> 
    Events.meminj_preserves_globals ge_S j -> 
    inject_incr j j' -> 
    Events.inject_separated j j' m1 m2 -> 
-   reserve_map_incr r r' -> 
-   reserve_map_separated r r' j' m1 m2 -> 
+   reserve_incr r r' -> 
+   reserve_separated r r' j' m1 m2 -> 
    Mem.inject j' m1' m2' -> 
    val_inject_opt j' retv1 retv2 -> 
    mem_forward m1 m1' -> 
    mem_forward m2 m2' -> 
-   Events.mem_unchanged_on (rely_left (csemS i) r d1) m1 m1' ->  
-   Events.mem_unchanged_on (rely_right (csemS i) j r d1) m2 m2' -> 
+   rely (csemS i) r d1 m1 m1' ->  
+   rely' (csemT i) j r d2 m2 m2' -> 
    val_has_type_opt' retv2 (proj_sig_res (ef_sig ef)) -> 
    after_external esemS retv1 s1 = Some s1' -> 
    after_external esemT retv2 s2 = Some s2' -> 
@@ -645,18 +662,19 @@ Module ExtendedSimulations. Section ExtendedSimulations.
    ACTIVE E_S s1 <> i -> 
    match_state i cd r' j' d1 m1' d2 m2')
 
-
- (make_initial_core_diagram: forall v1 vals1 s1 m1 v2 vals2 m2 r j sig,
+ (make_initial_core_diagram: forall v1 vals1 s1 m1 v2 vals2 m2 (r: reserve) j sig,
    In (v1, v2, sig) entry_points -> 
    make_initial_core esemS ge_S v1 vals1 = Some s1 -> 
    Mem.inject j m1 m2 -> 
-   reserve_map_valid r m1 -> 
-   reserve_map_valid_right r j m2 -> 
+   mem_wd m1 -> 
+   mem_wd m2 -> 
+   reserve_valid r m1 -> 
+   reserve_valid' r j m2 -> 
    Forall2 (val_inject j) vals1 vals2 -> 
    Forall2 Val.has_type vals2 (sig_args sig) -> 
    exists cd, exists s2, 
-                make_initial_core esemT ge_T v2 vals2 = Some s2 /\
-                match_states cd r j s1 m1 s2 m2)
+     make_initial_core esemT ge_T v2 vals2 = Some s2 /\
+     match_states cd r j s1 m1 s2 m2)
  
  (safely_halted_step: forall cd r j c1 m1 c2 m2 v1 rty,
    match_states cd r j c1 m1 c2 m2 -> 
@@ -673,18 +691,18 @@ Module ExtendedSimulations. Section ExtendedSimulations.
    PROJ_CORE E_T (ACTIVE E_S s1) s2 = Some c2 -> 
    safely_halted (csemS (ACTIVE E_S s1)) c1 = Some rv1 -> 
    corestep esemS ge_S s1 m1 s1' m1' ->  
+   guarantee esemS r s1' m1' -> 
    exists rv2, 
      safely_halted (csemT (ACTIVE E_S s1)) c2 = Some rv2 /\
      val_inject j rv1 rv2 /\ 
-   exists s2', exists m2', exists cd', exists r', exists j', 
-     inject_incr j j' /\
-     Events.inject_separated j j' m1 m2 /\
-     reserve_map_incr r r' /\
-     reserve_map_separated r r' j' m1 m2 /\
-     corestep esemT ge_T s2 m2 s2' m2' /\
-     match_states cd' r' j' s1' m1' s2' m2' /\
-     Events.mem_unchanged_on (guarantee_left (csemS (ACTIVE E_S s1)) r c1) m1 m1' /\
-     Events.mem_unchanged_on (guarantee_right (csemS (ACTIVE E_S s1)) j r c1) m2 m2'),
+     exists s2', exists m2', exists cd', exists r': reserve, exists j', 
+       inject_incr j j' /\
+       Events.inject_separated j j' m1 m2 /\
+       reserve_incr r r' /\
+       reserve_separated r r' j' m1 m2 /\
+       corestep esemT ge_T s2 m2 s2' m2' /\
+       match_states cd' r' j' s1' m1' s2' m2' /\
+       guarantee' esemT j' r' s2' m2'),
   internal_compilability_invariant.
 
  Variables 
@@ -696,28 +714,99 @@ Module ExtendedSimulations. Section ExtendedSimulations.
   (owned_conservS: owned_conserving esemS csemS E_S)
   (owned_conservT: owned_conserving esemT csemT E_T)
   (active_okS: (forall x_s, ACTIVE E_S x_s < max_cores)%nat)
-  (active_okT: (forall x_t, ACTIVE E_T x_t < max_cores)%nat).
+  (active_okT: (forall x_t, ACTIVE E_T x_t < max_cores)%nat)
+  (new_effects_alignedT: new_effects_aligned esemT csemT genv_mapT E_T).
 
 Program Definition extended_simulation: 
   Forward_simulation_inject D_S D_T esemS esemT ge_S ge_T 
            entry_points core_datas match_states (core_ords max_cores) :=
   @Build_Forward_simulation_inject _ _ _ _ _ _ _ 
   esemS esemT ge_S ge_T entry_points core_datas match_states (core_ords max_cores) 
-  _ _ _ _ _ _ _.
+  _ _ _ _ _ _ _ _ _ _ _ _.
 Next Obligation. apply core_ords_wf. Qed.
-Next Obligation.
+Next Obligation. 
+unfold match_states in H.
+destruct H as [? [? [? [? [RMV1 [RMV2 [? [? [WD1 [WD2 ?]]]]]]]]]].
+solve[split; auto].
+Qed.
+Next Obligation. 
 unfold match_states in H.
 destruct H as [? [? [? [? [RMV1 [RMV2 ?]]]]]].
 solve[split; auto].
 Qed.
 Next Obligation. 
-rename H0 into MATCH.
+unfold match_states in H.
+destruct H as [? [? [? [? [RMV1 [RMV2 [EV1 [EV2 [WD1 [WD2 ?]]]]]]]]]].
+solve[split; auto].
+Qed.
+Next Obligation. 
+unfold match_states in H.
+destruct H as [? [? [? [? [RMV1 [RMV2 [EV1 [EV2 [WD1 [WD2 [? [? [JJ ?]]]]]]]]]]]]].
+solve[eapply JJ; eauto].
+Qed.
+Next Obligation. 
+unfold match_states in H|-*. 
+destruct H as [? [? [? [? [RMV1 [RMV2 [EV1 [EV2 [WD1 [WD2 [? [? [JJ [RR ?]]]]]]]]]]]]]].
+repeat split3; auto.
+clear - RMV1 H0.
+intros b ofs RR.
+solve[apply(RMV1 b ofs (H0 _ _ RR))].
+clear - RMV2 H0.
+unfold reserve_valid' in RMV2|-*.
+intros until delta; intros H1 H2.
+solve[apply (RMV2 _ _ _ _ (H0 _ _ H1) H2)].
+solve[eapply guarantee_decr; eauto].
+clear - H5 H0.
+unfold guarantee'.
+intros b ofs V INJ EFM.
+specialize (H5 b ofs V).
+destruct INJ as [b0 [delta0 [H6 H7]]].
+apply H5; auto.
+solve[exists b0, delta0; split; auto].
+solve[eapply R_antimonotone; eauto].
+destruct H6 as [H6 [H7 H8]].
+solve[auto].
+destruct H6 as [H6 [H7' H8]].
+specialize (H7' _ H7).
+destruct H7'.
+solve[eapply guarantee_decr; eauto].
+destruct H6 as [H6 [H7' H8]].
+specialize (H7' _ H7).
+destruct H7' as [? [[z ?]]].
+exists z; auto.
+admit. (*compile_safe_decr*)
+destruct H6 as [H6 [H7' H8]].
+destruct (H7' _ H7) as [? [? [c2 [? [? ?]]]]].
+exists c2; split; auto.
+split.
+solve[eapply guarantee_decr2; eauto].
+solve[eapply match_antimono; eauto].
+destruct H6 as [H6 [H7 H8]].
+intros i c1 H9 H10.
+specialize (H8 _ _ H9 H10).
+destruct H8 as [c2 [PROJ [? [? [? [? [? MATCH]]]]]]].
+exists c2; split; auto.
+solve[exists x, x0, x1, x2, x3; auto].
+Qed.
+Next Obligation.
+destruct H as 
+ [? [? [? [? [RMV1 [RMV2 [EV1 [EV2 [WD1 [WD2 [? [? [JJ [RR [? [MATCH1 MATCH2]]]]]]]]]]]]]]]].
+destruct (active_proj_core E_S c1) as [c2' H7].
+specialize (MATCH1 _ H7).
+destruct MATCH1 as [GR [c3 [PROJ [? [GR2 MATCH]]]]].
+solve[eapply match_validblocks in MATCH; eauto].
+Qed.
+Next Obligation. 
+rename H0 into G0.
+rename H1 into MATCH.
 generalize MATCH as MATCH'; intro.
-destruct MATCH as [VAL1 [DISJ1 [VAL2 [DISJ2 [RVAL1 [RVAL2 [RR [ACT MATCH_CORES]]]]]]]].
+destruct MATCH as [VAL1 [DISJ1 [VAL2 [DISJ2 [RVAL1 [RVAL2 
+ [EV1 [EV2 [WD1 [WD2 [GR1 [GR2 [JJ [RR [ACT [MATCH_CORES1 MATCH_CORES2]]]]]]]]]]]]]]]].
 rename H into STEP.
 destruct (active_proj_core E_S st1) as [c1 PROJ1].
 destruct (active_proj_core E_T st2) as [c2 PROJ2].
-assert (exists c2':cT (ACTIVE E_S st1), PROJ_CORE E_T (ACTIVE E_S st1) st2 = Some c2').
+assert (exists c2':cT (ACTIVE E_S st1), 
+  PROJ_CORE E_T (ACTIVE E_S st1) st2 = Some c2').
  clear - ACT c2 PROJ2.
  forget (ACTIVE E_S st1) as xx.
  forget (ACTIVE E_T st2) as yy.
@@ -732,11 +821,12 @@ intros RUN1.
 assert (RUN2: runnable (csemT (ACTIVE E_S st1)) c2=true).
  inv esig_compilable.
  rewrite match_state_runnable 
-  with (cd := cd (ACTIVE E_S st1)) (r := r) (j := j) (m1 := m1) (c2 := c2) (m2 := m2) in RUN1.
+  with (cd := cd (ACTIVE E_S st1)) (r := r) (j := j) 
+       (m1 := m1) (c2 := c2) (m2 := m2) in RUN1.
  auto.
- specialize (MATCH_CORES (ACTIVE E_S st1) c1).
- spec MATCH_CORES; auto.
- destruct MATCH_CORES as [c2' [PROJ2' MTCH]].
+ specialize (MATCH_CORES1 c1).
+ spec MATCH_CORES1; auto.
+ destruct MATCH_CORES1 as [GRc1 [SAFE [c2' [PROJ2' [GRc2 MTCH]]]]].
  rewrite PROJ2' in PROJ2.
  inv PROJ2.
  solve[auto].
@@ -763,11 +853,25 @@ assert (ACT1': ACTIVE E_S st1 = ACTIVE E_S st1').
  solve[destruct corestep_pres; auto].
 generalize (core_diagram (core_simulations (ACTIVE E_S st1))) as DIAG; intro.
 clear c2 PROJ2 RUN2.
-destruct (MATCH_CORES (ACTIVE E_S st1) c1 PROJ1) as [c2 [PROJ2 MATCH12]].
+destruct (MATCH_CORES1 c1 PROJ1) as [GRc1 [SAFE [c2 [PROJ2 [GRc2 MATCH12]]]]].
 unfold core_datas in cd.
-specialize (DIAG c1 m1 c1' m1' STEP1 (cd _) r c2 j m2 MATCH12).
+assert (G_INNER: guarantee (csemS (ACTIVE E_S st1)) r c1' m1').
+ destruct SAFE as [z SAFE].
+ apply compile_safe_safe' in SAFE.
+ specialize (SAFE (S O)).
+ hnf in SAFE.
+ assert (AT_EXT: at_external (csemS (ACTIVE E_S st1)) c1 = None).
+  solve[eapply corestep_not_at_external; eauto].
+ rewrite AT_EXT in SAFE.
+ assert (HALT: safely_halted (csemS (ACTIVE E_S st1)) c1 = None).
+  solve[eapply corestep_not_halted; eauto].
+ rewrite HALT in SAFE.
+ destruct (SAFE _ _ STEP1) as [r' [INCR [SEP [GR _]]]].
+ solve[eapply guarantee_decr; eauto].
+ admit. (*corestep_fun*)
+specialize (DIAG c1 m1 c1' m1' STEP1 (cd _) r c2 j m2 G_INNER MATCH12).
 destruct DIAG as [c2' [m2' [cd' [r' [j' [INJ_INCR [INJ_SEP [RINCR [RSEP 
- [MATCH12' [UNCH1 [UNCH2 STEP2]]]]]]]]]]]].
+ [UNCH2 [MATCH12' STEP2]]]]]]]]]]].
 destruct STEP2 as [STEP2|STEP2].
 
 (*corestep_plus case*)
@@ -787,6 +891,19 @@ split3; auto.
 split; auto.
 split; auto.
 split; auto.
+forget (ACTIVE E_S st1) as x.
+forget (ACTIVE E_T st2') as y.
+subst.
+eapply (guarantee_stepN owned_conservT new_effects_alignedT); eauto.
+intros b ofs ? ? delta b2 ?.
+specialize (RSEP b ofs).
+spec RSEP; auto.
+spec RSEP; auto.
+destruct RSEP as [_ H2].
+solve[eapply H2; eauto].
+intros b ofs ? ? ?.
+solve[exploit (INJ_SEP b ofs); eauto; intros [X Y]; apply Y; auto].
+split; auto.
  (*Subgoal: match_states*)
  hnf.
  split.
@@ -795,6 +912,7 @@ split; auto.
  eapply owned_valid_inv with (n := S O); eauto.
  solve[simpl; exists c1'; exists m1'; eauto].
  solve[simpl; eexists st1'; eexists m1'; eauto].
+
  (*owned_disjoint*)
  split.
  eapply owned_disjoint_inv with (n := S O) (m' := m1'); eauto.
@@ -807,6 +925,7 @@ split; auto.
  forget (ACTIVE E_T st2') as k2.
  subst.
  solve[eapply owned_valid_inv; eauto].
+
  (*owned_disjoint*)
  split.
  forget (ACTIVE E_S st1) as k1.
@@ -814,15 +933,54 @@ split; auto.
  subst.
  solve[eapply owned_disjoint_inv; eauto].
 
+ (*reserve_valid*)
  split.
  destruct (core_simulations (ACTIVE E_S st1)).
- eapply reserve_valid0 in MATCH12'.
+ eapply reserved_locs_valid0 in MATCH12'.
  solve[destruct MATCH12'; auto].
  split.
  destruct (core_simulations (ACTIVE E_S st1)).
- eapply reserve_valid0 in MATCH12'.
+ eapply reserved_locs_valid0 in MATCH12'.
  solve[destruct MATCH12'; auto].
 
+ (*effects_valid*)
+ split.
+ admit. 
+ split.
+ admit.
+
+ (*mem_wd*)
+ split.
+ admit.
+ split.
+ admit.
+ 
+ (*guarantee*)
+ split.
+ eapply guarantee_incr_alloc1; eauto.
+ eapply reserved_locs_valid in MATCH12'; eauto.
+ destruct MATCH12'; auto.
+ solve[intros b1 ofs1 X Y; destruct (RSEP b1 ofs1); auto].
+ split.
+ forget (ACTIVE E_S st1) as x.
+ subst.
+ eapply (guarantee_stepN owned_conservT new_effects_alignedT); eauto.
+ intros b ofs ? ? delta b2 ?.
+ specialize (RSEP b ofs).
+ spec RSEP; auto.
+ spec RSEP; auto.
+ destruct RSEP as [_ H2].
+ solve[eapply H2; eauto].
+ intros b ofs ? ? ?.
+ solve[exploit (INJ_SEP b ofs); eauto; intros [X Y]; apply Y; auto].
+  
+ (*allocs_shrink*)
+ split.
+ unfold allocs_shrink.
+ intros until delta; intros EFA2 JJ'.
+ admit. (*TODO*)
+
+ (*R*)
  split.
  inv esig_compilable. 
  eapply corestep_rel with (s1 := st1) (s2 := st2); eauto.
@@ -830,28 +988,37 @@ split; auto.
  erewrite meminj_preserves_genv2blocks.
  eauto.
  solve[apply genvs_domain_eq_sym; auto].
+ solve[eapply guarantee_decr2; eauto].
 
  split.
- solve[rewrite <-ACT1', <-ACT2'; auto].
- 
-  intros i _c _PROJ1'.
-  case_eq (eq_nat_dec (ACTIVE E_S st1) i).
-  
+  solve[rewrite <-ACT1', <-ACT2'; auto].
+  split. 
+
   (*ACTIVE E_S st1 = i*)
+  intros _c _PROJ1'.
   forget (ACTIVE E_S st1) as x.
   forget (ACTIVE E_T st2) as y.
   forget (ACTIVE E_S st1') as x'.
   forget (ACTIVE E_T st2') as y'.
-  intros EQ _. 
   do 4 subst.
+  assert (_c = c1') as ->.
+   rewrite PROJ1' in _PROJ1'.
+   solve[inv _PROJ1'; auto].
+  split.
+  eapply guarantee_incr_alloc1; eauto.
+  eapply reserved_locs_valid in MATCH12'; eauto.
+  solve[destruct MATCH12'; auto].
+  intros b1 ofs1 ? ?.
+  solve[destruct (RSEP b1 ofs1); auto].
+  split.
+  admit. (*compile_safety*)
   exists c2'.
-  rewrite PROJ1' in _PROJ1'.
-  inv _PROJ1'.
+  split; auto.
   split; auto.
   solve[unfold core_datas_upd; rewrite data_upd_same; auto].
 
   (*ACTIVE E_S st1 <> i*)
-  intros NEQ _.
+  intros i _c NEQ PROJ.
   assert (_PROJ1: PROJ_CORE E_S i st1 = Some _c). 
    inv core_compatS.
    specialize (corestep_others_forward st1 st1'). 
@@ -865,11 +1032,14 @@ split; auto.
    spec corestep_others_forward; auto. 
    spec corestep_others_forward; auto.
    spec corestep_others_forward; auto.
-   specialize (corestep_others_forward i NEQ).
+   specialize (corestep_others_forward i).
+   spec corestep_others_forward; auto.
    solve[rewrite corestep_others_forward; auto].
-  assert (exists _d, PROJ_CORE E_T i st2 = Some _d) as [_d _PROJ2].
-   destruct (MATCH_CORES i _c _PROJ1) as [_d [_PROJ2 _MATCH12]].
-   solve[exists _d; auto].
+  specialize (MATCH_CORES2 i _c).
+  spec MATCH_CORES2.
+  solve[rewrite ACT1'; auto].
+  destruct (MATCH_CORES2 _PROJ1) as 
+   [_d [_PROJ2 [cd0 [r0 [j0 [m10 [m20 [GR10 [GR20 _MATCH12]]]]]]]]].
   assert (_PROJ2': PROJ_CORE E_T i st2' = Some _d). 
    inv core_compatT.
    specialize (corestep_others_backward st2). 
@@ -882,43 +1052,11 @@ split; auto.
    spec corestep_others_backward; auto.
    spec corestep_others_backward; auto. 
    spec corestep_others_backward; auto.
-   specialize (corestep_others_backward i NEQ).
+   specialize (corestep_others_backward i).
+   spec corestep_others_backward; auto.
    solve[rewrite <-corestep_others_backward; auto].
   exists _d; split; auto.
-  inv esig_compilable.
-  specialize (match_others i cd r r' j j' st1 cd' c1 m1 c1' m1' st2 c2 m2 c2' m2' _c _d (S n)).
-  unfold core_datas_upd; rewrite data_upd_other; auto.
-  apply match_others; auto.
-   solve[eapply match_state_inj; eauto].
-   erewrite <-genvs_domain_eq_preserves.
-   erewrite meminj_preserves_genv2blocks.
-   eauto.
-   solve[apply genvs_domain_eq_sym; auto].
-
-   split.
-   (*mem_unch_on unmapped*)
-   apply mem_unchanged_on_sub with (Q := 
-    guarantee_left (csemS (ACTIVE E_S st1)) r c1); auto.
-   intros b ofs [X Y]; split; auto.
-   intros CONTRA; apply Y.
-   assert (owned (csemS (ACTIVE E_S st1)) c1 b ofs -> 
-           owned esemS st1 b ofs).
-    solve[apply owned_conservS; auto].
-   solve[auto].
-   split.
-   apply mem_unchanged_on_sub with (Q := 
-     guarantee_right (csemS (ACTIVE E_S st1)) j r c1); auto.
-   intros b ofs [b' [delta [X [Y W]]]].
-   unfold guarantee_right.
-   exists b'; exists delta.
-   split; auto.
-   split; auto.
-   intros CONTRA; apply W.
-   assert (owned (csemS (ACTIVE E_S st1)) c1 b' (ofs-delta) -> 
-           owned esemS st1 b' (ofs-delta)).
-    solve[apply owned_conservS; auto].
-   solve[auto].
-
+  solve[exists cd0, r0, j0, m10, m20; split; auto].
   solve[left; exists n; auto].
 
 (*corestep_star case*)
@@ -936,19 +1074,29 @@ exists r'.
 exists j'.
 split3; auto.
 split; auto.
+split; auto.
+split; auto.
+forget (ACTIVE E_S st1) as x.
+subst.
+eapply (guarantee_stepN owned_conservT new_effects_alignedT); eauto.
+intros b ofs ? ? delta b2 ?.
+specialize (RSEP b ofs).
+spec RSEP; auto.
+spec RSEP; auto.
+destruct RSEP as [_ H2].
+solve[eapply H2; eauto].
+intros b ofs ? ? ?.
+solve[exploit (INJ_SEP b ofs); eauto; intros [X Y]; apply Y; auto].
+split.
  (*Subgoal: match_states*)
  hnf.
  split.
 
- (*reserve_map_separated*)
- solve[auto].
-
- split.
- split.
  (*owned_valid*)
  eapply owned_valid_inv with (n := S O); eauto.
  solve[simpl; exists c1'; exists m1'; eauto].
  solve[simpl; eexists st1'; eexists m1'; eauto].
+
  (*owned_disjoint*)
  split.
  eapply owned_disjoint_inv with (n := S O) (m' := m1'); eauto.
@@ -961,6 +1109,7 @@ split; auto.
  forget (ACTIVE E_T st2') as k2.
  subst.
  solve[eapply owned_valid_inv; eauto].
+
  (*owned_disjoint*)
  split.
  forget (ACTIVE E_S st1) as k1.
@@ -968,15 +1117,54 @@ split; auto.
  subst.
  solve[eapply owned_disjoint_inv; eauto].
 
+ (*reserve_valid*)
  split.
  destruct (core_simulations (ACTIVE E_S st1)).
- eapply reserve_valid0 in MATCH12'.
+ eapply reserved_locs_valid0 in MATCH12'.
  solve[destruct MATCH12'; auto].
  split.
  destruct (core_simulations (ACTIVE E_S st1)).
- eapply reserve_valid0 in MATCH12'.
+ eapply reserved_locs_valid0 in MATCH12'.
  solve[destruct MATCH12'; auto].
 
+ (*effects_valid*)
+ split.
+ admit.
+ split.
+ admit.
+
+ (*mem_wd*)
+ split.
+ admit.
+ split.
+ admit.
+
+ (*guarantee*)
+ split.
+ eapply guarantee_incr_alloc1; eauto.
+ eapply reserved_locs_valid in MATCH12'; eauto.
+ destruct MATCH12'; auto.
+ solve[intros b1 ofs1 X Y; destruct (RSEP b1 ofs1); auto].
+ split.
+ forget (ACTIVE E_S st1) as x.
+ subst.
+ eapply (guarantee_stepN owned_conservT new_effects_alignedT); eauto.
+ intros b ofs ? ? delta b2 ?.
+ specialize (RSEP b ofs).
+ spec RSEP; auto.
+ spec RSEP; auto.
+ destruct RSEP as [_ H2].
+ solve[eapply H2; eauto].
+ intros b ofs ? ? ?.
+ solve[exploit (INJ_SEP b ofs); eauto; intros [X Y]; apply Y; auto].
+ 
+ (*allocs_shrink*)
+ split.
+ unfold allocs_shrink.
+ intros until delta; intros EFA2 JJ'.
+ admit. (*TODO*)
+
+ (*R*)
  split.
  inv esig_compilable. 
  eapply corestep_rel with (s1 := st1) (s2 := st2); eauto.
@@ -984,28 +1172,37 @@ split; auto.
  erewrite meminj_preserves_genv2blocks.
  eauto.
  solve[apply genvs_domain_eq_sym; auto].
+ solve[eapply guarantee_decr2; eauto].
 
  split.
- solve[rewrite <-ACT2'; auto].
+  solve[rewrite <-ACT1', <-ACT2'; auto].
+  split. 
 
-  intros i _c _PROJ1'.
-  case_eq (eq_nat_dec (ACTIVE E_S st1) i).
-  
   (*ACTIVE E_S st1 = i*)
+  intros _c _PROJ1'.
   forget (ACTIVE E_S st1) as x.
   forget (ACTIVE E_T st2) as y.
   forget (ACTIVE E_S st1') as x'.
   forget (ACTIVE E_T st2') as y'.
-  intros EQ _. 
   do 4 subst.
+  assert (_c = c1') as ->.
+   rewrite PROJ1' in _PROJ1'.
+   solve[inv _PROJ1'; auto].
+  split.
+  eapply guarantee_incr_alloc1; eauto.
+  eapply reserved_locs_valid in MATCH12'; eauto.
+  solve[destruct MATCH12'; auto].
+  intros b1 ofs1 ? ?.
+  solve[destruct (RSEP b1 ofs1); auto].
+  split.
+  admit. (*compile_safe*)
   exists c2'.
-  rewrite PROJ1' in _PROJ1'.
-  inv _PROJ1'.
+  split; auto.
   split; auto.
   solve[unfold core_datas_upd; rewrite data_upd_same; auto].
 
   (*ACTIVE E_S st1 <> i*)
-  intros NEQ _.
+  intros i _c NEQ _PROJ1'.
   assert (_PROJ1: PROJ_CORE E_S i st1 = Some _c). 
    inv core_compatS.
    specialize (corestep_others_forward st1 st1'). 
@@ -1019,11 +1216,14 @@ split; auto.
    spec corestep_others_forward; auto. 
    spec corestep_others_forward; auto.
    spec corestep_others_forward; auto.
-   specialize (corestep_others_forward i NEQ).
+   specialize (corestep_others_forward i).
+   spec corestep_others_forward; auto.
    solve[rewrite corestep_others_forward; auto].
-  assert (exists _d, PROJ_CORE E_T i st2 = Some _d) as [_d _PROJ2].
-   destruct (MATCH_CORES i _c _PROJ1) as [_d [_PROJ2 _MATCH12]].
-   solve[exists _d; auto].
+  specialize (MATCH_CORES2 i _c).
+  spec MATCH_CORES2.
+  solve[rewrite ACT1'; auto].
+  destruct (MATCH_CORES2 _PROJ1) as 
+   [_d [_PROJ2 [cd0 [r0 [j0 [m10 [m20 [GR10 [GR20 _MATCH12]]]]]]]]].
   assert (_PROJ2': PROJ_CORE E_T i st2' = Some _d). 
    inv core_compatT.
    specialize (corestep_others_backward st2). 
@@ -1036,44 +1236,12 @@ split; auto.
    spec corestep_others_backward; auto.
    spec corestep_others_backward; auto. 
    spec corestep_others_backward; auto.
-   specialize (corestep_others_backward i NEQ).
+   specialize (corestep_others_backward i).
+   spec corestep_others_backward; auto.
    solve[rewrite <-corestep_others_backward; auto].
   exists _d; split; auto.
-  inv esig_compilable.
-  specialize (match_others i cd r r' j j' st1 cd' c1 m1 c1' m1' st2 c2 m2 c2' m2' _c _d n).
-  unfold core_datas_upd; rewrite data_upd_other; auto.
-  apply match_others; auto.
-  solve[eapply match_state_inj; eauto].
-  erewrite <-genvs_domain_eq_preserves.
-  erewrite meminj_preserves_genv2blocks.
-  solve[eapply match_state_preserves_globals; eauto].
-  solve[apply genvs_domain_eq_sym; auto].
-
-  split. 
-  (*mem_unch_on unmapped*)
-   apply mem_unchanged_on_sub with (Q := 
-    guarantee_left (csemS (ACTIVE E_S st1)) r c1); auto.
-   intros b ofs [X Y]; split; auto.
-   intros CONTRA; apply Y.
-   assert (owned (csemS (ACTIVE E_S st1)) c1 b ofs -> 
-           owned esemS st1 b ofs).
-    solve[apply owned_conservS; auto].
-   solve[auto].
-   split.
-   apply mem_unchanged_on_sub with (Q := 
-     guarantee_right (csemS (ACTIVE E_S st1)) j r c1); auto.
-   intros b ofs [b' [delta [X [Y W]]]].
-   unfold guarantee_right.
-   exists b'; exists delta.
-   split; auto.
-   split; auto.
-   intros CONTRA; apply W.
-   assert (owned (csemS (ACTIVE E_S st1)) c1 b' (ofs-delta) -> 
-           owned esemS st1 b' (ofs-delta)).
-    solve[apply owned_conservS; auto].
-   solve[auto].
-
-  right. split. exists n. auto. 
+  solve[exists cd0, r0, j0, m10, m20; split; auto].
+  right. split. exists n. auto.
   solve[apply core_datas_upd_ord; auto].
 
 (*runnable = false*)
@@ -1084,10 +1252,9 @@ apply runnable_false in RUN1.
 destruct RUN1 as [[rv1 HALT]|[ef [sig [args AT_EXT]]]].
 
 (*active thread is safely halted*)
-specialize (MATCH_CORES (ACTIVE E_S st1) c1 _PROJ1).
+specialize (MATCH_CORES1 c1 _PROJ1).
 clear c2 PROJ2.
-destruct MATCH_CORES as [c2 [PROJ2 MATCH12]].
-
+destruct MATCH_CORES1 as [GRc1 [SAFE [c2 [PROJ2 [GRc2 MATCH12]]]]].
 destruct (exists_ty rv1) as [ty1 HAS_TY].
 destruct (core_halted (core_simulations (ACTIVE E_S st1)) 
   (cd (ACTIVE E_S st1)) r j c1 m1 c2 m2 rv1 ty1 MATCH12 HALT) 
@@ -1096,39 +1263,24 @@ inv esig_compilable.
 eapply safely_halted_diagram with (m1' := m1') in MATCH'; eauto.
 destruct MATCH' as [rv2' [H7 [VAL_INJ' 
  [st2' [m2' [cd' [r' [j' [INJ_INCR [SEP [STEP2' 
- [RM_INCR [RM_SEP [MATCH12' [UNCH1 UNCH2]]]]]]]]]]]]]]].
+ [RM_INCR [RM_SEP [MATCH12' UNCH2]]]]]]]]]]]]]].
 exists st2'; exists m2'; exists cd'; exists r'; exists j'.
 split3; auto; split; auto.
 split3; auto.
-
-split.
-apply mem_unchanged_on_sub with (Q := 
-  guarantee_left (csemS (ACTIVE E_S st1)) r c1); auto.
-intros b ofs [? ?]; split; auto.
-intros CONTRA.
-apply H0.
-solve[eapply owned_conservS in CONTRA; eauto].
-
-split.
-apply mem_unchanged_on_sub with (Q := 
-  guarantee_right (csemS (ACTIVE E_S st1)) j r c1); auto.
-intros b ofs [? [? [? [? ?]]]].
-exists x; exists x0; split; auto.
 split; auto.
-intros CONTRA.
-apply H1.
-solve[eapply owned_conservS in CONTRA; eauto].
-
 solve[left; exists 0%nat; eexists; eexists; split; simpl; eauto].
 
 (*active thread is at_external*)
 clear c2 PROJ2.
-destruct (MATCH_CORES (ACTIVE E_S st1) c1 _PROJ1) as [c2 [PROJ2 MATCH12]].
+destruct (MATCH_CORES1 c1 _PROJ1) as [GRc1 [SAFE [c2 [GRc2 [PROJ2 MATCH12]]]]].
 destruct (core_at_external (core_simulations (ACTIVE E_S st1)) (cd (ACTIVE E_S st1)) 
             r j c1 m1 c2 m2 ef args sig MATCH12 AT_EXT)
- as [H6 [H7 [vals2 [H8 [H9 H10]]]]].
+ as [H6 [H7 [vals2 [H8 [H9 [H10 H11]]]]]].
+
+admit. (*forall v1 : val, In v1 args -> val_valid v1 m1*)
+
 inv esig_compilable. 
-edestruct extension_diagram as [s2' H11]; eauto.
+edestruct extension_diagram as [s2' H12]; eauto.
 solve[erewrite <-match_state_runnable; eauto].
 rewrite <-meminj_preserves_genv2blocks.
 rewrite genvs_domain_eq_preserves with (ge2 := (genv_mapS (ACTIVE E_S st1))); auto.
@@ -1143,43 +1295,50 @@ Next Obligation. inv esig_compilable. eapply safely_halted_step; eauto. Qed.
 Next Obligation. 
 rename H into MATCH.
 hnf in MATCH.
-destruct MATCH as [PRIV1 [DISJ1 [PRIV2 [DISJ2 [RMV1 [RMV2 [RR [ACT MATCH_CORES]]]]]]]].
+destruct MATCH 
+ as [PRIV1 [DISJ1 [PRIV2 [DISJ2 [RMV1 [RMV2 [EV1 [EV2 
+    [WD1 [WD2 [GR1 [GR2 [SHRINK [RR [ACT [MATCH_CORES1 MATCH_CORES2]]]]]]]]]]]]]]]].
 destruct (active_proj_core E_S) with (s := st1) as [c1 PROJ1].
 assert (AT_EXT1: at_external (csemS (ACTIVE E_S st1)) c1 = Some (e, sig, vals1)).
  inv core_compatS.
  edestruct (at_extern_call) as [c [PROJ AT_EXT]]; eauto.
  rewrite PROJ in PROJ1; inv PROJ1.
  solve[inv PROJ; auto].
-destruct (MATCH_CORES (ACTIVE E_S st1) c1 PROJ1) as [c2 [PROJ2 MATCH12]].
+destruct (MATCH_CORES1 c1 PROJ1) as [GRc1 [SAFE [c2 [PROJ2 [GRc2 MATCH12]]]]].
 destruct (core_at_external (core_simulations (ACTIVE E_S st1)) 
             (cd (ACTIVE E_S st1)) r j c1 m1 c2 m2 e vals1 sig MATCH12 AT_EXT1)
- as [INJ [GLOBS [vals2 [VALINJ [TYPE AT_EXT2]]]]].
+ as [INJ [GLOBS [vals2 [VALINJ [TYPE [AT_EXT2 VALVAL]]]]]].
+solve[apply H1].
 split3; auto.
 rewrite <-meminj_preserves_genv2blocks.
 rewrite genvs_domain_eq_preserves with (ge2 := (genv_mapS (ACTIVE E_S st1))); auto.
 rewrite meminj_preserves_genv2blocks; auto.
 exists vals2.
 split3; auto.
+split; auto.
 inv esig_compilable.
 eapply at_external_match; eauto.
 rewrite <-meminj_preserves_genv2blocks.
 rewrite genvs_domain_eq_preserves with (ge2 := (genv_mapS (ACTIVE E_S st1))); auto.
-rewrite meminj_preserves_genv2blocks; auto.
+solve[rewrite meminj_preserves_genv2blocks; auto].
 Qed.
 
-Next Obligation. 
-rename H0 into MATCH.
+Next Obligation.
+rename H into MATCH.
 generalize MATCH as MATCH'; intro.
 hnf in MATCH.
-destruct MATCH as [PRIV1 [DISJ1 [PRIV2 [DISJ2 [RMV1 [RMV2 [RR [ACT MATCH_CORES]]]]]]]].
-generalize MATCH_CORES as MATCH_CORES'; intro.
+destruct MATCH 
+ as [PRIV1 [DISJ1 [PRIV2 [DISJ2 [RMV1 [RMV2 
+    [EV1 [EV2 [WD1 [WD2 [GR1 [GR2 [SHRINK [RR 
+    [ACT [MATCH_CORES1 MATCH_CORES2]]]]]]]]]]]]]]]].
+generalize MATCH_CORES2 as MATCH_CORES'; intro.
 destruct (active_proj_core E_S) with (s := st1) as [c1 PROJ1].
 assert (AT_EXT1: at_external (csemS (ACTIVE E_S st1)) c1 = Some (e, sig, vals1)).
  inv core_compatS.
  edestruct (at_extern_call) as [c [PROJ AT_EXT]]; eauto.
  rewrite PROJ in PROJ1; inv PROJ1.
  solve[inv PROJ; auto].
-destruct (MATCH_CORES (ACTIVE E_S st1) c1 PROJ1) as [c2 [PROJ2 MATCH12]].
+destruct (MATCH_CORES1 c1 PROJ1) as [GRc1 [SAFE [c2 [PROJ2 [GRc2 MATCH12]]]]].
 destruct (core_after_external (core_simulations (ACTIVE E_S st1)) 
                 (cd (ACTIVE E_S st1)) r r' j j' c1 c2 m1 e 
                 vals1 ret1 m1' m2 m2' ret2 sig)
@@ -1188,16 +1347,21 @@ rewrite <-meminj_preserves_genv2blocks.
 rewrite <-genvs_domain_eq_preserves with (ge1 := ge_S); auto.
 rewrite meminj_preserves_genv2blocks; auto.
 
-apply mem_unchanged_on_sub with (Q := rely_left esemS r st1); auto.
+unfold rely in H13|-*.
+apply mem_unchanged_on_sub with (Q := fun b ofs => 
+  r b ofs /\ effects esemS st1 AllocEffect b ofs); auto.
 intros b ofs [? ?].
 split; auto.
 solve[eapply owned_conservS; eauto].
-apply mem_unchanged_on_sub with (Q := rely_right esemS j r st1); auto.
-intros b ofs [? [? [? [? ?]]]].
+unfold rely', rely in H14|-*.
+apply mem_unchanged_on_sub with (Q := fun b ofs => 
+  inject_reserve j r b ofs /\ effects esemT st2 AllocEffect b ofs); auto.
+unfold inject_reserve.
+intros b ofs [[? [? [? ?]]] EF].
+split.
 exists x, x0.
 split; auto.
-split; auto.
-solve[eapply owned_conservS; eauto].
+solve[eapply owned_conservT; eauto].
 
 exists (core_datas_upd (ACTIVE E_S st1) cd' cd).
 assert (exists st1', after_external esemS ret1 st1 = Some st1' /\
@@ -1206,7 +1370,7 @@ assert (exists st1', after_external esemS ret1 st1 = Some st1' /\
  specialize (after_ext_prog st1 c1 c1' ret1).
  solve[spec after_ext_prog; auto].
 assert (exists st2', after_external esemT ret2 st2 = Some st2' /\
-         PROJ_CORE E_T (ACTIVE E_S st1) st2' = Some c2') as [st2' [? PROJ2']].
+   PROJ_CORE E_T (ACTIVE E_S st1) st2' = Some c2') as [st2' [? PROJ2']].
  inv core_compatT.
  specialize (after_ext_prog st2). 
  rewrite <-ACT in after_ext_prog.
@@ -1228,102 +1392,170 @@ split; auto.
 (*owned_valid*)
 solve[eapply owned_valid_after_ext; eauto].
 split.
+
 (*owned_disjoint*)
 solve[eapply owned_disjoint_after_ext; eauto].
 split.
+
 (*owned_valid*)
 remember (ACTIVE E_S st1) as x.
 remember (ACTIVE E_S st1') as x'.
 remember (ACTIVE E_T st2') as y'.
 subst.
 assert (AT_EXT2: exists vals2, 
- at_external (csemT (ACTIVE E_T st2)) c2 = Some (e, sig, vals2)).
+  Forall2 (val_inject j) vals1 vals2 /\
+  Forall2 (Val.has_type) vals2 (sig_args (ef_sig e)) /\
+  at_external (csemT (ACTIVE E_T st2)) c2 = Some (e, sig, vals2) /\
+  (forall v2, In v2 vals2 -> val_valid v2 m2)).
  destruct (core_simulations (ACTIVE E_T st2)).
  eapply core_at_external0 in AT_EXT1; eauto.
- destruct AT_EXT1 as [_ [_ [vals2 [_ [_ AT_EXT2]]]]].
- exists vals2; eauto.
- destruct AT_EXT2 as [vals2 AT_EXT2].
- solve[eapply owned_valid_after_ext; eauto].
+ destruct AT_EXT1 as [_ [_ [vals2 [X [Y [AT_EXT2 VALVAL]]]]]].
+ solve[exists vals2; eauto].
+destruct AT_EXT2 as [vals2 [FV1 [FV2 [AT_EXT2 VALVAL]]]].
+solve[eapply owned_valid_after_ext; eauto].
+
 (*owned_disjoint*)
 remember (ACTIVE E_S st1) as x.
 remember (ACTIVE E_S st1') as x'.
 remember (ACTIVE E_T st2') as y'.
 subst.
 assert (AT_EXT2: exists vals2, 
- at_external (csemT (ACTIVE E_T st2)) c2 = Some (e, sig, vals2)).
+  Forall2 (val_inject j) vals1 vals2 /\
+  Forall2 (Val.has_type) vals2 (sig_args (ef_sig e)) /\
+  at_external (csemT (ACTIVE E_T st2)) c2 = Some (e, sig, vals2) /\
+  (forall v2, In v2 vals2 -> val_valid v2 m2)).
  destruct (core_simulations (ACTIVE E_T st2)).
  eapply core_at_external0 in AT_EXT1; eauto.
- destruct AT_EXT1 as [_ [_ [vals2 [_ [_ AT_EXT2]]]]].
- exists vals2; eauto.
-destruct AT_EXT2 as [vals2 AT_EXT2].
+ destruct AT_EXT1 as [_ [_ [vals2 [X [Y [AT_EXT2 VALVAL]]]]]].
+ solve[exists vals2; eauto].
 split.
+destruct AT_EXT2 as [vals2 [FV1 [FV2 [AT_EXT2 VALVAL]]]].
 solve[eapply owned_disjoint_after_ext; eauto].
 
+(*reserve_valid_after_ext*)
 split.
 destruct (core_simulations (ACTIVE E_T st2)).
-eapply reserve_valid0 in MATCH12'.
+eapply reserved_locs_valid0 in MATCH12'.
 solve[destruct MATCH12'; auto].
 split.
 destruct (core_simulations (ACTIVE E_T st2)).
-eapply reserve_valid0 in MATCH12'.
+eapply reserved_locs_valid0 in MATCH12'.
 solve[destruct MATCH12'; auto].
+
+(*effects_valid_after_ext*)
+split.
+admit.
+split. 
+admit.
+
+(*mem_wd_after_ext*)
+split; auto.
+split; auto.
+
+(*guarantee_after_ext*)
+split. 
+admit.
+split. 
+admit.
+
+(*allocs_shrink_after_ext*)
+split.
+unfold allocs_shrink.
+admit.
 
 split.
 inv esig_compilable.
 eapply after_external_rel; eauto.
-split; auto.
+eapply rely_same_effects; eauto.
+solve[intros; eapply effects_external; eauto].
+unfold rely', rely in H14|-*.
+apply mem_unchanged_on_sub with (Q := 
+  (fun b ofs => inject_reserve j r b ofs /\ 
+    effects esemT st2 AllocEffect b ofs)); auto.
+intros b ofs [? ?]; split; auto.
+assert (exists vals2, at_external esemT st2 = Some (e, sig, vals2))
+    as [vals2 AT_EXT2'].
+ destruct AT_EXT2 as [vals2 [FV1 [FV2 [AT_EXT2 VALVAL]]]].
+ exists vals2.
+ remember (ACTIVE E_T st2) as y.
+ forget (ACTIVE E_S st1') as x'.
+ forget (ACTIVE E_T st2') as y'.
+ do 4 subst.
+ specialize (at_external_match 
+    st1 m1 st2 c1 c2 m2 e sig vals1 vals2 (cd (ACTIVE E_S st1)) r j).
+ spec at_external_match; auto.
+ spec at_external_match; auto.
+ spec at_external_match; auto.
+ spec at_external_match; auto.
+ solve[eapply match_state_runnable; eauto].
+ spec at_external_match; auto.
+ spec at_external_match; auto.
+ spec at_external_match; auto.
+ spec at_external_match; auto.
+ solve[eapply match_state_inj; eauto].
+solve[intros; eapply effects_external; eauto].
 
-intros i _c _PROJ1'.
-case_eq (eq_nat_dec (ACTIVE E_S st1) i).
+split; auto.
+split.
 (*ACTIVE E_S st1 = i*)
 forget (ACTIVE E_S st1) as x.
 forget (ACTIVE E_T st2) as y.
 forget (ACTIVE E_S st1') as x'.
 forget (ACTIVE E_T st2') as y'.
 do 4 subst.
-intros EQ _; subst.
-exists c2'; split; auto.
+intros _c _PROJ1'.
 rewrite _PROJ1' in PROJ1'.
 inv PROJ1'; auto.
+split.
+eapply guarantee_after_ext; eauto.
+eapply effects_valid in MATCH12; eauto.
+solve[destruct MATCH12; auto].
+intros b ofs; intros.
+rename H6 into RSEP.
+specialize (RSEP b ofs).
+spec RSEP; auto.
+spec RSEP; auto.
+destruct RSEP as [RSEP _]; auto.
+split.
+(*compile_safe*)
+destruct SAFE as [z SAFE].
+assert (HALT: safely_halted (csemS x') c1 = None).
+ exploit @at_external_halted_excl; eauto.
+ instantiate (1 := c1).
+ instantiate (1 := (csemS x')).
+ intros [X|X].
+ rewrite X in AT_EXT1; congruence.
+ solve[auto].
+inv SAFE; try solve[congruence].
+solve[apply corestep_not_at_external in H21; congruence].
+exists z.
+eapply H19; eauto.
+intros b ofs ? ? ?.
+solve[apply (H6 b ofs); auto].
+admit. (*val_not_reserved; will have to be added to after_external*)
+exists c2'.
+split; auto.
+split; auto.
+admit. (*guarantee'_incr_after_external*)
 solve[unfold core_datas_upd; rewrite data_upd_same; auto].
 
 (*ACTIVE E_S st1 <> i*)
-intros NEQ _.
+intros i _c NEQ _PROJ1'.
 specialize (MATCH_CORES' i _c).
+spec MATCH_CORES'; auto.
+rewrite Heqx in NEQ.
 spec MATCH_CORES'.
  inv core_compatS.
  solve[erewrite after_ext_others; eauto].
 destruct MATCH_CORES' as [_d [_PROJ2 _MATCH12]].
 exists _d; split; auto.
- inv core_compatT.
- erewrite <-after_ext_others; eauto.
- solve[rewrite Heqx; auto].
-unfold core_datas_upd; rewrite data_upd_other; auto.
-inv esig_compilable.
-eapply after_external_diagram; eauto.
-inv core_compatS.
-erewrite <-after_ext_others in _PROJ1'; eauto.
-apply mem_unchanged_on_sub with (Q := rely_left esemS r st1); auto.
-intros b ofs [? ?].
-split; auto.
-apply owned_conservS in _PROJ1'.
-solve[eapply _PROJ1'; eauto].
-apply mem_unchanged_on_sub with (Q := rely_right esemS j r st1); auto.
-intros b ofs [? [? [? [? ?]]]].
-exists x; exists x0; split; auto.
-split; auto.
-assert (PROJ_CORE E_S i st1 = Some _c).
- inv core_compatS.
- solve[erewrite after_ext_others; eauto].
-solve[eapply owned_conservS in H18; eauto].
 inv core_compatT.
 erewrite <-after_ext_others; eauto.
-solve[rewrite Heqx; auto].
 solve[rewrite Heqx; auto].
 Qed.
 
 Lemma RGsimulations_invariant: 
-  (forall i:nat, StableRelyGuaranteeSimulation.Sig (csemS i) (csemT i) 
+  (forall i:nat, RelyGuaranteeSimulation.Sig (csemS i) (csemT i) 
        (genv_mapS i) (match_state i)) ->
   @CompilabilityInvariant.Sig F_S V_S F_T V_T D_S D_T xS xT 
        fS fT vS vT cS cT dS dT Z Zint Zext 
@@ -1332,61 +1564,15 @@ Lemma RGsimulations_invariant:
        entry_points core_data match_state core_ord R -> 
   internal_compilability_invariant.
 Proof.
-intro core_simulations_RGinject.
-constructor; try solve[inv H; auto].
-  
-(*1*)
-intros until n; intros PROJC1 PROJC2 PROJD1 PROJD2 ACT MATCH INJ PRES INCR 
- SEP RMI1 RMSEP2 STEP1 STEP2 MATCHC' UNCH1 UNCH2.
-destruct MATCH as [PRIV1 [DISJ1 [PRIV2 [DISJ2 [RM1 [RM2 [RR [ACTEQ MATCH_INNER]]]]]]]].
-forget (Extension.active E_S s1) as k.
-destruct (MATCH_INNER k c1 PROJC1) as [_c2 [_PROJC2 MATCHC]].
-rewrite _PROJC2 in PROJC2; inv PROJC2.
-destruct (MATCH_INNER i d1 PROJD1) as [_d2 [_PROJD2 MATCHD]].
-rewrite _PROJD2 in PROJD2; inv PROJD2.
-forget (Extension.active E_T s2) as k.
-destruct (core_simulations_RGinject k) as [_ ? ? _ _].
-destruct (core_simulations_RGinject i) as [_ _ _ RELY _].
-specialize (RELY (genv_mapS i) (cd i) m1 m1' r r' j j' m2 m2' d1 d2).
-apply RELY; auto.
-erewrite <-genvs_domain_eq_preserves; eauto.
-solve[eapply match_state_inj; eauto].
-apply mem_unchanged_on_sub with (Q := guarantee_left (csemS k) r c1); auto.
-intros b ofs [X Y].
-split; auto.
-solve[unfold owned_disjoint in DISJ1; eapply DISJ1; eauto].
-apply mem_unchanged_on_sub with (Q := guarantee_right (csemS k) j r c1); auto.
-intros b ofs [b' [delta [X [Y W]]]].
-exists b'; exists delta; split; auto.
-split; auto.
-intros CONTRA.
-solve[unfold owned_disjoint in DISJ1; eapply DISJ1; eauto].
-
-(*2*)
-intros; destruct (core_simulations_RGinject i) as [? _ _ _ _].
+intros core_simulations_RGinject INV.
+inv INV.
+constructor; auto.
+intros; destruct (core_simulations_RGinject i) as [? _ _].
 eapply match_state_runnable; eauto.
-
-(*3*)
-intros; destruct (core_simulations_RGinject i) as [_ ? _ _ _].
+intros; destruct (core_simulations_RGinject i) as [_ ? _].
 solve[eapply match_state_inj; eauto].
-
-(*4*)
-intros; destruct (core_simulations_RGinject i) as [_ _ ? _ _].
+intros; destruct (core_simulations_RGinject i) as [_ _ ?].
 solve[eapply match_state_preserves_globals; eauto].
-
-(*5*)
-intros until j'; intros MATCH EXT1 PRES INCR SEP RM RMSEP 
- INJ INJARGS FORW1 UNCH1 FORW2 UNCH2.
-intros TYS AFTER1 AFTER2 PROJ1 PROJ2 NEQ.
-forget (Extension.active E_S s1) as k.
-destruct (core_simulations_RGinject i) as [? ? ? RELY].
-specialize (RELY (genv_mapS i) cd m1 m1' r r' j j' m2 m2' d1 d2).
-apply RELY; auto.
-solve[eapply match_state_inj; eauto].
-erewrite genvs_domain_eq_preserves.
-erewrite meminj_preserves_genv2blocks.
-eauto.
-solve[apply genvs_domain_eq_sym; auto].
 Qed.
 
 End ExtendedSimulations. End ExtendedSimulations.
@@ -1402,12 +1588,12 @@ Module ExtensionCompilability. Section ExtensionCompilability.
   (Z: Type) (** external states *)
   (Zint: Type) (** portion of Z implemented by extension *)
   (Zext: Type) (** portion of Z external to extension *)
-  (esemS: RelyGuaranteeSemantics (Genv.t F_S V_S) xS D_S) (** extended source semantics *)
-  (esemT: RelyGuaranteeSemantics (Genv.t F_T V_T) xT D_T) (** extended target semantics *)
+  (esemS: EffectfulSemantics (Genv.t F_S V_S) xS D_S) (** extended source semantics *)
+  (esemT: EffectfulSemantics (Genv.t F_T V_T) xT D_T) (** extended target semantics *)
   (csemS: forall i:nat, 
-    RelyGuaranteeSemantics (Genv.t (fS i) (vS i)) (cS i) (dS i)) (** a set of core semantics *)
+    EffectfulSemantics (Genv.t (fS i) (vS i)) (cS i) (dS i)) (** a set of core semantics *)
   (csemT: forall i:nat, 
-    RelyGuaranteeSemantics (Genv.t (fT i) (vT i)) (cT i) (dT i)) (** a set of core semantics *)
+    EffectfulSemantics (Genv.t (fT i) (vT i)) (cT i) (dT i)) (** a set of core semantics *)
   (csig: ef_ext_spec mem Z) (** client signature *)
   (esig: ef_ext_spec mem Zext) (** extension signature *)
   (threads_max: nat).
@@ -1425,7 +1611,7 @@ Module ExtensionCompilability. Section ExtensionCompilability.
  Variable entry_points: list (val*val*signature).
  Variable core_data: forall i: nat, Type.
  Variable match_state: forall i: nat, 
-   core_data i -> reserve_map -> meminj -> cS i -> mem -> cT i -> mem -> Prop.
+   core_data i -> reserve -> meminj -> cS i -> mem -> cT i -> mem -> Prop.
  Variable core_ord: forall i: nat, core_data i -> core_data i -> Prop.
  Implicit Arguments match_state [].
  Implicit Arguments core_ord [].
@@ -1433,7 +1619,12 @@ Module ExtensionCompilability. Section ExtensionCompilability.
 
  Definition core_datas := forall i: nat, core_data i. 
 
- Variable R: reserve_map -> meminj -> xS -> mem -> xT -> mem -> Prop.
+ Variable R: reserve -> meminj -> xS -> mem -> xT -> mem -> Prop.
+ Variable R_antimono: 
+   forall (r0 r: reserve) j s1 m1 s2 m2,
+   reserve_incr r0 r -> 
+   R r j s1 m1 s2 m2 -> 
+   R r0 j s1 m1 s2 m2.
 
  Import Forward_simulation_inj_exposed.
 
@@ -1443,11 +1634,12 @@ Module ExtensionCompilability. Section ExtensionCompilability.
        E_S E_T entry_points core_data match_state core_ord R.
  Proof.
  eapply @EXTENSION_COMPILABILITY.Make.
- intros H1 H2 H3 H4 H5 H6 PRIV1 PRIV2 core_simulations H8 H9 H10.
+ intros H1 H2 H3 H4 H5 H6 PRIV1 PRIV2 core_simulations H8 H9 H10 H11.
  apply CompilableExtension.Make 
   with (core_datas := ExtendedSimulations.core_datas core_data)
        (match_states := 
-  ExtendedSimulations.match_states fS fT vS vT esemS esemT csemS csemT E_S E_T match_state R)
+  ExtendedSimulations.match_states fS fT vS vT esemS esemT csemS csemT 
+                                   genv_mapS E_S E_T match_state R)
        (core_ords := 
   ExtendedSimulations.core_ords core_data core_ord max_cores).
  eapply ExtendedSimulations.extended_simulation; eauto.
@@ -1469,16 +1661,17 @@ Module ExtensionCompilability2. Section ExtensionCompilability2.
   (Z: Type) (** external states *)
   (Zint: Type) (** portion of Z implemented by extension *)
   (Zext: Type) (** portion of Z external to extension *)
-  (esemS: RelyGuaranteeSemantics (Genv.t F_S V_S) cS D_S) (** extended source semantics *)
-  (esemT: RelyGuaranteeSemantics (Genv.t F_T V_T) cT D_T) (** extended target semantics *)
-  (csemS: RelyGuaranteeSemantics (Genv.t fS vS) cS dS)
-  (csemT: RelyGuaranteeSemantics (Genv.t fT vT) cT dT)
+  (esemS: EffectfulSemantics (Genv.t F_S V_S) cS D_S) (** extended source semantics *)
+  (esemT: EffectfulSemantics (Genv.t F_T V_T) cT D_T) (** extended target semantics *)
+  (csemS: EffectfulSemantics (Genv.t fS vS) cS dS)
+  (csemT: EffectfulSemantics (Genv.t fT vT) cT dT)
   (csig: ef_ext_spec mem Z) (** client signature *)
   (esig: ef_ext_spec mem Zext) (** extension signature *)
   (handled: list AST.external_function). (** functions handled by this extension *)
 
  Variables 
-  (ge_S: Genv.t F_S V_S) (ge_T: Genv.t F_T V_T) (geS: Genv.t fS vS) (geT: Genv.t fT vT).
+  (ge_S: Genv.t F_S V_S) (ge_T: Genv.t F_T V_T) 
+  (geS: Genv.t fS vS) (geT: Genv.t fT vT).
 
  Variable (E_S: @Extension.Sig mem Z Zint Zext (Genv.t F_S V_S) D_S cS esemS esig 
    _ _ (const cS) (const csemS) csig). 
@@ -1486,7 +1679,8 @@ Module ExtensionCompilability2. Section ExtensionCompilability2.
    _ _ (const cT) (const csemT) csig). 
  Variable entry_points: list (val*val*signature).
  Variable core_data: Type.
- Variable match_state: core_data -> reserve_map -> meminj -> cS -> mem -> cT -> mem -> Prop.
+ Variable match_state: 
+   core_data -> reserve -> meminj -> cS -> mem -> cT -> mem -> Prop.
  Variable core_ord: core_data -> core_data -> Prop.
  Implicit Arguments match_state [].
  Implicit Arguments core_ord [].
@@ -1494,7 +1688,12 @@ Module ExtensionCompilability2. Section ExtensionCompilability2.
 
  Definition core_datas := nat -> core_data.
 
- Variable R: reserve_map -> meminj -> cS -> mem -> cT -> mem -> Prop.
+ Variable R: reserve -> meminj -> cS -> mem -> cT -> mem -> Prop.
+ Variable R_antimono: 
+   forall (r0 r: reserve) j s1 m1 s2 m2,
+   reserve_incr r0 r -> 
+   R r j s1 m1 s2 m2 -> 
+   R r0 j s1 m1 s2 m2.
 
  Import Forward_simulation_inj_exposed.
 
@@ -1505,15 +1704,16 @@ Module ExtensionCompilability2. Section ExtensionCompilability2.
     (const match_state) (const core_ord) R.
  Proof.
  eapply @EXTENSION_COMPILABILITY.Make.
- intros H1 H2 H3 H4 H5 H6 PRIV1 PRIV2 core_simulations H8 H9 H10.
+ intros H1 H2 H3 H4 H5 H6 PRIV1 PRIV2 core_simulations H8 H9 H10 INV.
  apply CompilableExtension.Make 
   with (core_datas := ExtendedSimulations.core_datas (fun _ => core_data))
        (match_states := 
   ExtendedSimulations.match_states (const fS) (const fT) (const vS) (const vT) 
-              esemS esemT (const csemS) (const csemT) E_S E_T (const match_state) R)
+              esemS esemT (const csemS) (const csemT) 
+              (const geS) E_S E_T (const match_state) R)
        (core_ords := 
   ExtendedSimulations.core_ords (const core_data) (const core_ord) max_cores).
- eapply ExtendedSimulations.extended_simulation; eauto.
+ eapply ExtendedSimulations.extended_simulation; eauto. 
  solve[eapply ExtendedSimulations.RGsimulations_invariant; eauto].
 Qed.
 
